common/LanguageInterface.v
@@ -248,6 +248,89 @@ Proof.
     eauto.
 Qed.
 
+(** ** Rectangular diagrams *)
+
+(** *** Extension passes *)
+
+Lemma match_cc_extends id sg vargs1 m1 vargs2 m2:
+  Mem.extends m1 m2 ->
+  Val.lessdef_list vargs1 vargs2 ->
+  exists w,
+    match_query (cc_c extp) w (cq id sg vargs1 m1) (cq id sg vargs2 m2) /\
+    forall vres1 m1' vres2 m2',
+      match_reply (cc_c extp) w (vres1, m1') (vres2, m2') ->
+      Val.lessdef vres1 vres2 /\
+      Mem.extends m1' m2' /\
+      Mem.unchanged_on (loc_out_of_bounds m1) m2 m2'.
+Proof.
+  intros Hm Hvargs.
+  exists (extpw m1 m2). split.
+  - constructor; simpl; eauto.
+    + exists 0. reflexivity.
+    + apply val_inject_list_lessdef in Hvargs.
+      induction Hvargs; constructor; eauto.
+    + constructor; eauto.
+  - intros vres1 m1' vres2 m2' (w' & Hw' & Hvres & Hm'). cbn [fst snd] in *.
+    inversion Hw' as [xm1 xm2 xm1' xm2' Hperm Hunch]; subst.
+    inv Hm'. simpl in Hvres. red in Hvres.
+    intuition eauto.
+    apply val_inject_lessdef; eauto.
+Qed.
+
+(** *** Injections *)
+
+Lemma match_cc_inject fb1 sg f vargs1 m1 fb2 vargs2 m2:
+  block_inject f fb1 fb2 ->
+  Val.inject_list f vargs1 vargs2 ->
+  Mem.inject f m1 m2 ->
+  exists w,
+    match_query (cc_c injp) w (cq fb1 sg vargs1 m1) (cq fb2 sg vargs2 m2) /\
+    forall vres1 m1' vres2 m2',
+      match_reply (cc_c injp) w (vres1, m1') (vres2, m2') ->
+      exists f',
+        Val.inject f' vres1 vres2 /\
+        Mem.inject f' m1' m2' /\
+        Mem.unchanged_on (loc_unmapped f) m1 m1' /\
+        Mem.unchanged_on (loc_out_of_reach f m1) m2 m2' /\
+        inject_incr f f' /\
+        inject_separated f f' m1 m2 /\
+        forall b ofs p,
+          Mem.valid_block m1 b ->
+          Mem.perm m1' b ofs Max p ->
+          Mem.perm m1 b ofs Max p.
+Proof.
+  intros Hfb Hvargs Hm.
+  exists (injpw f m1 m2). simpl. split.
+  - constructor; simpl; eauto.
+    induction Hvargs; constructor; eauto.
+  - intros vres1 m1' vres2 m2' (w' & Hw' & Hvres & Hm'). simpl in *.
+    inv Hw'. inv Hm'.
+    exists f'. intuition eauto.
+    destruct (f b) as [[b' delta] | ] eqn:Hb.
+    + eauto.
+    + eapply Mem.unchanged_on_perm; eauto.
+Qed.
+
+(** For passes which use a triangular injection diagram for their
+  incoming calls, the following lemma may be useful for proving the
+  [block_inject] premise of [match_cc_inject]. *)
+
+Lemma funct_ptr_flat_inject {F V} (ge: Genv.t F V) f fd b thr:
+  Genv.find_funct_ptr ge b = Some fd ->
+  Block.le Block.init thr ->
+  inject_incr (Mem.flat_inj thr) f ->
+  block_inject f b b.
+Proof.
+  clear.
+  intros Hfd Hthr Hf.
+  apply Genv.find_funct_ptr_iff in Hfd.
+  apply Genv.genv_defs_range in Hfd.
+  exists 0. apply Hf.
+  unfold Mem.flat_inj.
+  destruct Block.lt_dec; eauto.
+  elim n. blomega.
+Qed.
+
 (** ** Triangular diagrams *)
 
 (** When proving simulation for initial and final states, we do not
@@ -272,6 +355,9 @@ Qed.
   rectangular diagram can be recovered. *)
 
 (** *** Extensions *)
+
+Definition cc_extends_triangle :=
+  cc_c_tr ext.
 
 (** The following lemma and tactic are used in simulation proofs for
   initial states, as a way to inverse the [match_query] hypothesis.
@@ -317,47 +403,62 @@ Qed.
 (** The triangular diagram for injections requires the initial
   memories and arguments to be "inject_neutral". *)
 
+Inductive cc_inject_triangle_mq: block -> query li_c -> query li_c -> Prop :=
+  cc_inject_triangle_mq_intro fb sg vargs m:
+    let f := Mem.flat_inj (Mem.nextblock m) in
+    block_inject f fb fb ->
+    Val.inject_list f vargs vargs ->
+    Mem.inject f m m ->
+    cc_inject_triangle_mq
+      (Mem.nextblock m)
+      (cq fb sg vargs m)
+      (cq fb sg vargs m).
+
+Definition cc_inject_triangle_mr nb: reply li_c -> reply li_c -> Prop :=
+  fun '(vres1, m1') '(vres2, m2') =>
+    exists f',
+      Val.inject f' vres1 vres2 /\
+      Mem.inject f' m1' m2' /\
+      inject_incr (Mem.flat_inj nb) f'.
+
+Definition cc_inject_triangle: callconv li_c li_c :=
+  {|
+    ccworld := block;
+    match_senv nb := symbols_inject (Mem.flat_inj nb);
+    match_query := cc_inject_triangle_mq;
+    match_reply := cc_inject_triangle_mr;
+  |}.
+
 (** The following lemma is used to prove initial state simulations,
   as a way to inverse the [match_query] hypothesis. See also the
   [inv_triangle_query] tactic below. *)
 
 Lemma match_query_cc_inject_triangle (P: _ -> _ -> _ -> _ -> _ -> _ -> Prop):
-  (forall id sg vargs m,
+  (forall fb sg vargs m,
+    block_inject (Mem.flat_inj (Mem.nextblock m)) fb fb ->
     Val.inject_list (Mem.flat_inj (Mem.nextblock m)) vargs vargs ->
     Mem.inject (Mem.flat_inj (Mem.nextblock m)) m m ->
-    P id sg vargs m (cq id sg vargs m) (cq id sg vargs m)) ->
+    P fb sg vargs m (cq fb sg vargs m) (cq fb sg vargs m)) ->
   (forall w q1 q2,
-    match_query (cc_c_tr inj) w q1 q2 ->
+    match_query cc_inject_triangle w q1 q2 ->
     P (cq_fb q1) (cq_sg q1) (cq_args q1) (cq_mem q1) q1 q2).
 Proof.
-  intros H w q1 q2 Hq.
-  destruct Hq as [q Hw [Hfb _ Hvargs Hm]].
-  destruct q as [fb sg vargs m]; simpl in *.
-  assert (w = Mem.flat_inj (Mem.nextblock m)).
-  {
-    apply Axioms.functional_extensionality; intros b1.
-    specialize (Hw b1).
-    unfold Mem.flat_inj in *.
-    destruct Block.lt_dec as [Hb|Hb]; eauto.
-    destruct (w b1) as [[b2 delta] | ] eqn:Hb'; eauto.
-    elim Hb. eapply Mem.valid_block_inject_1; eauto.
-  }
-  subst.
+  intros H m q1 q2 Hq.
+  destruct Hq as [fb sg vargs f Hfb Hvargs Hm]; simpl in *.
   apply H; auto.
-  apply val_inject_list_rel; auto.
 Qed.
 
 (** The following lemma is used in simulation proofs for final states,
   to show that corresponding replies are related. *)
 
-Lemma match_reply_cc_inject_triangle f f' vres1 m1' vres2 m2':
+Lemma match_reply_cc_inject_triangle nb f' vres1 m1' vres2 m2':
   Val.inject f' vres1 vres2 ->
   Mem.inject f' m1' m2' ->
-  inject_incr f f' ->
-  match_reply (cc_c_tr inj) f (vres1, m1') (vres2, m2').
+  inject_incr (Mem.flat_inj nb) f' ->
+  match_reply cc_inject_triangle nb (vres1, m1') (vres2, m2').
 Proof.
   intros Hvres Hm' Hf'.
-  exists f'; split; rauto.
+  exists f'; eauto.
 Qed.
 
 (** *** Tactics *)
@@ -371,6 +472,7 @@ Ltac inv_triangle_query :=
   let q2 := fresh "q2" in
   let Hq := fresh "Hq" in
   intros w q1 q2 Hq;
+  try replace w with (Mem.nextblock (cq_mem q1)) by (inv Hq; eauto);
   pattern (cq_fb q1), (cq_sg q1), (cq_args q1), (cq_mem q1), q1, q2;
   revert w q1 q2 Hq;
   first
